qweqwe

DList.fst
@@ -45,7 +45,7 @@ type dlisthead (t:Type) = {
 }
 
 (** Be able to use [null] very very easily *)
-inline_for_extraction abstract private
+inline_for_extraction private unfold
 let null #t = null t
 
 (** Initialze an element of a doubly linked list *)
@@ -58,7 +58,9 @@ let empty_list (#t:Type) : dlisthead t =
 
 unfold let op_At_Bang (#t:Type) (h0:mem) (p:pointer t) = Buffer.get h0 p 0
 unfold let op_String_Access = Seq.index
-unfold let not_null a = ~(is_null a)
+unfold let not_null (#t:Type) (a:pointer_or_null t) = Buffer.length a <> 0
+
+let _ = assert_norm (forall (t:Type) (p:pointer_or_null t). is_null p \/ not_null p)
 
 unfold
 let dlisthead_is_valid (#t:Type) (h0:mem) (h:dlisthead t) =
@@ -69,14 +71,15 @@ let dlisthead_is_valid (#t:Type) (h0:mem) (h:dlisthead t) =
   (empty <==> is_null h.lhead) /\
   (~empty ==> (is_null (h0@! h.lhead).blink) /\
               (is_null (h0@! h.ltail).flink) /\
+              (live h0 h.lhead /\ live h0 h.ltail) /\
               (h0@! h.ltail == nodes.[l-1]) /\
               (h0@! h.lhead == nodes.[0]) /\
               (forall i. {:pattern (nodes.[i]).blink}
-                 ((1 <= i /\ i < Seq.length nodes) ==>
+                 ((1 <= i /\ i < l) ==>
                   not_null (nodes.[i]).blink /\
                   h0@! (nodes.[i]).blink == nodes.[i-1])) /\
               (forall i. {:pattern (nodes.[i]).flink}
-                 ((0 <= i /\ i < Seq.length nodes - 1) ==>
+                 ((0 <= i /\ i < l - 1) ==>
                   not_null (nodes.[i]).flink /\
                   h0@! (nodes.[i]).flink == nodes.[i+1])))
 
@@ -87,65 +90,53 @@ let dlist_is_member_of (#t:eqtype) (h0:mem) (e:pointer (dlist t)) (h:dlisthead t
   Seq.mem (h0@! e) (Ghost.reveal h.nodes)
 
 unfold inline_for_extraction
-let (<&) (#t:Type) (p:pointer t) (x:t)
-  // : ST unit
-  //   (fun h0 -> live h0 p)
-  //   (fun h1 () h2 -> modifies_1 p h1 h2 /\ h2@! p == x /\ live h2 p)
-  =
+let (<&) (#t:Type) (p:pointer t) (x:t) =
   p.(0ul) <- x
 
-unfold
 let erased_single_node (#t:eqtype) (e:pointer (dlist t)) =
   hide (Seq.create 1 !*e)
 
-#set-options "--z3rlimit 50"
+// #set-options "--z3rlimit 1" // Forces it to quickly hit resource bounds and then --detail_errors seems to get it through ¯\_(ツ)_/¯
+
+#set-options "--max_fuel 64 --max_ifuel 64 --z3rlimit 10"
+
+let createSingletonList (#t:eqtype) (e:pointer (dlist t)): ST (dlisthead t)
+    (requires (fun h0 -> live h0 e))
+    (ensures (fun h1 y h2 -> modifies_1 e h1 h2 /\ live h2 e /\ dlisthead_is_valid h2 y)) =
+  let h1 = ST.get () in
+  e <& { !*e with flink=null; blink = null }; // isn't this inefficient?
+  let y = { lhead = e; ltail = e; nodes = erased_single_node e } in
+  let h2 = ST.get () in
+  assert (is_null (h2@! e).flink /\
+          is_null (h2@! e).blink);
+  assert (y.lhead == e /\ y.ltail == e);
+  assert (Seq.length (Ghost.reveal y.nodes) == 1);
+  assert (live h2 e);
+  assert (live h2 y.lhead /\ live h2 y.ltail);
+  assert (h2@! y.lhead == (Ghost.reveal y.nodes).[0]);
+  assert (h2@! y.ltail == (Ghost.reveal y.nodes).[0]);
+  assert ((forall i. {:pattern ((Ghost.reveal y.nodes).[i]).blink}
+             ((1 <= i /\ i < 1) ==>
+              not_null ((Ghost.reveal y.nodes).[i]).blink /\
+              h2@! ((Ghost.reveal y.nodes).[i]).blink == (Ghost.reveal y.nodes).[i-1])) );
+  assert ((forall i. {:pattern ((Ghost.reveal y.nodes).[i]).flink}
+             ((0 <= i /\ i < 0) ==>
+              not_null ((Ghost.reveal y.nodes).[i]).flink /\
+              h2@! ((Ghost.reveal y.nodes).[i]).flink == (Ghost.reveal y.nodes).[i+1])));
+  assert (dlisthead_is_valid h2 y);
+  assert (live h2 e);
+  assert (modifies_1 e h1 h2);
+  assert (modifies_1 e h1 h2 /\ live h2 e /\ dlisthead_is_valid h2 y);
+  y
+
 
 (** Insert an element e as the first element in a doubly linked list *)
 let insertHeadList (#t:eqtype) (h:dlisthead t) (e:pointer (dlist t)): ST (dlisthead t)
    (requires (fun h0 -> dlisthead_is_valid h0 h /\ live h0 e /\ ~(dlist_is_member_of h0 e h)))
-   (ensures (fun _ y h2 -> dlisthead_is_valid h2 y))
+   (ensures (fun _ y h2 -> live h2 e /\ dlisthead_is_valid h2 y))
 =
   if is_null h.lhead then ( // the list is empty
-    e.(0ul) <- { e.(0ul) with flink=null; blink = null }; // isn't this inefficient?
-    // e <& { !*e with flink=null; blink = null }; // isn't this inefficient?
-    let h1' = ST.get () in
-    let y : dlisthead t = { lhead = e; ltail = e; nodes = erased_single_node e } in
-    // let h2 = ST.get () in assert ( dlisthead_is_valid h2 y ); // not sure why F* needs this coaxing
-    let h2 = ST.get () in
-    assert (h1' == h2);
-    // admit ();
-    // assert (dlist_is_member_of h2 e y);
-    // admit ();
-    assert (
-      let nodes = Ghost.reveal y.nodes in
-      let l = Seq.length nodes in
-      let empty : bool = l = 0 in
-      (~empty) /\
-      True);
-    admit ();
-    assert (
-      let nodes = Ghost.reveal y.nodes in
-      let l = Seq.length nodes in
-      let empty = l = 0 in
-      (empty <==> is_null y.ltail) /\
-      // (empty <==> is_null y.lhead) /\
-      // (~empty ==> (is_null (h2@! y.lhead).blink) /\
-      //             (is_null (h2@! y.ltail).flink) /\
-      //             (h2@! y.ltail == nodes.[l-1]) /\
-      //             (h2@! y.lhead == nodes.[0]) /\
-      //             (forall i. {:pattern (nodes.[i]).blink}
-      //                ((1 <= i /\ i < Seq.length nodes) ==>
-      //                 not_null (nodes.[i]).blink /\
-      //                 h2@! (nodes.[i]).blink == nodes.[i-1])) /\
-      //             (forall i. {:pattern (nodes.[i]).flink}
-      //                ((0 <= i /\ i < Seq.length nodes - 1) ==>
-      //                 not_null (nodes.[i]).flink /\
-      //                 h2@! (nodes.[i]).flink == nodes.[i+1])) /\
-      //             True
-      // ) /\
-      True
-    );
-    y
+    createSingletonList e
   ) else (
     let next = h.lhead in
     admit ();
@@ -154,85 +145,6 @@ let insertHeadList (#t:eqtype) (h:dlisthead t) (e:pointer (dlist t)): ST (dlisth
     let ghoste = hide !*e in
     let y = { lhead = e; ltail = h.ltail; nodes = elift2 Seq.cons ghoste h.nodes } in
     let h2 = ST.get () in assert ( dlisthead_is_valid h2 y );
+    admit ();
     y
   )
-
-(*
-(** Insert an element e as the last element in a doubly linked list. *)
-let insertTailList (#t:Type) (h:dlisthead t) (e:pointer (dlist t)): ST (dlisthead t)
-   (requires (fun h0 -> dlisthead_is_valid h0 h /\ live h0 e))
-   (ensures (fun _ y h2 -> dlisthead_is_valid h2 y))
-=
-  if is_null h.lhead then ( // the list is empty
-    e.(0ul) <- { !*e with flink=null; blink = null };
-    { lhead = e; ltail = e; nodes = hide (Seq.create 1 !*e) }
-  ) else (
-    let prev = h.ltail in
-    prev.(0ul) <- { !*prev with flink=e; }; // tail->flink=e
-    e.(0ul) <- { !*e with flink=null; blink = prev }; // e->flink=null/e.blink=tail
-    let ghoste = hide !*e in
-    { lhead = h.lhead; ltail = e; nodes = elift2 Seq.snoc h.nodes ghoste }
-  )
-
-(** Remove entry e from the doubly linked list *)
-let removeEntryList (#t:eqtype) (h:dlisthead t) (e:pointer (dlist t)): ST (dlisthead t)
-    (requires (fun h0 -> dlisthead_is_valid h0 h /\ not (is_null h.lhead) /\ live h0 e /\
-         (h.lhead == e <==> is_null ((get h0 e 0).blink)) /\
-         (h.ltail == e <==> is_null ((get h0 e 0).flink)) /\
-         live h0 (get h0 e 0).blink /\
-         live h0 (get h0 e 0).flink))
-   (ensures (fun _ y h2 -> dlisthead_is_valid h2 y))
-=
-  if ptr_eq h.lhead e then ( // removing from the head of the list
-    if ptr_eq h.ltail e then (// and removing from the tail - the list will now be empty
-      { lhead = null; ltail = null; nodes = hide Seq.createEmpty }
-    ) else (
-      let next = (!*e).flink in
-      next.(0ul) <- { next.(0ul) with blink = null; }; // e.flink.blink <- null
-      admit ();
-      { lhead = (!*e).flink; ltail = h.ltail; nodes = elift1 Seq.tail h.nodes }
-    )
-  ) else if ptr_eq h.ltail e then ( // removing from the tail of the list, but the list will be non-empty
-    let prev = (!*e).blink in
-    prev.(0ul) <- { prev.(0ul) with flink = null; }; // e.blink.flink <- null
-    admit ();
-    { lhead = h.lhead; ltail = (!*e).blink; nodes = elift1 fst (elift1 Seq.Properties.un_snoc h.nodes) }
-  ) else ( // removing from the middle of the list
-    let next = (!*e).flink in
-    let prev = (!*e).blink in
-    prev.(0ul) <- { prev.(0ul) with flink = next; };
-    next.(0ul) <- { next.(0ul) with blink = prev; };
-    admit ();
-    h // TODO: Write down a { h with nodes = REMOVE !*e FROM h.nodes } here
-  )
-
-(** Insert e after prior, in list h *)
-let insertEntryAfter (#t:Type) (h:dlisthead t) (prior:pointer (dlist t)) (e:pointer (dlist t)): ST (dlisthead t)
-   (requires (fun _ -> true))
-   (ensures (fun _ _ _ -> true))
-=
-  if ptr_eq h.ltail prior then ( // appending to the end of the list
-    insertTailList h e
-  ) else (
-    let next = (!*prior).flink in
-    prior.(0ul) <- { prior.(0ul) with flink = e };
-    e.(0ul) <- { e.(0ul) with blink=prior; flink=next };
-    next.(0ul) <- { next.(0ul) with blink = e };
-    h
-  )
-
-(** Insert e after next, in list h *)
-let insertEntryBefore (#t:Type) (h:dlisthead t) (next:pointer (dlist t)) (e:pointer (dlist t)): ST (dlisthead t)
-   (requires (fun _ -> true))
-   (ensures (fun _ _ _ -> true))
-=
-  if h.lhead = next then ( // adding to the front of the list
-    insertHeadList h e
-  ) else (
-    let prior = (!*next).blink in
-    prior.(0ul) <- { prior.(0ul) with flink = e };
-    e.(0ul) <- { e.(0ul) with blink=prior; flink=next };
-    next.(0ul) <- { next.(0ul) with blink = e };
-    h
-  )
-*)
